BusyLean/BusyLean.lean
@@ -2,3 +2,5 @@ import BusyLean.Defs
 import BusyLean.TapeHelpers
 import BusyLean.Parser
 import BusyLean.RunLemmas
+import BusyLean.Notation
+import BusyLean.Tactics
